updates

Veritas.EAC.fst
@@ -7,59 +7,79 @@ open Veritas.Key
 open Veritas.MultiSetHash
 open Veritas.Record
 open Veritas.SeqAux
+open Veritas.SeqMachine
 open Veritas.State
+open Veritas.StateSeqMachine
 open Veritas.Verifier
 
 //Allow the solver to unroll recursive functions at most once (fuel)
 //Allow the solver to invert inductive definitions at most once (ifuel)
 #push-options "--max_fuel 1 --max_ifuel 1 --initial_fuel 1 --initial_ifuel 1"
 
+let is_evict (e: vlog_entry) = 
+  match e with
+  | EvictM _ _ -> true
+  | EvictB _ _ -> true
+  | EvictBM _ _ _ -> true
+  | _ -> false
+
+type evict_vlog_entry = e:vlog_entry {is_evict e}
+type nevict_vlog_entry = e:vlog_entry {not (is_evict e)}
+
+type vlog_entry_ext =
+  | NEvict: e:nevict_vlog_entry -> vlog_entry_ext
+  | Evict: e:evict_vlog_entry -> v:value -> vlog_entry_ext
+
+type vlog_ext = seq (vlog_entry_ext)
+
 type eac_state = 
   | EACFail: eac_state  
   | EACInit: eac_state
-  | EACInCache: m:add_method -> k:key -> v:value -> eac_state
-  | EACEvicted: m:add_method -> k:key -> v:value -> eac_state
+  | EACInCache: m:add_method -> v:value -> eac_state
+  | EACEvicted: m:add_method -> v:value -> eac_state
 
-let eac_add (e: vlog_entry) (s: eac_state) : eac_state = 
+let eac_add (e: vlog_entry_ext) (s: eac_state) : eac_state = 
   match s with
   | EACFail -> EACFail
   | EACInit -> (
     match e with 
-    | AddM (k,v) _ -> if v = init_value k then EACInCache MAdd k v
-                      else EACFail
+    | NEvict (AddM (k,v) _) -> if v = init_value k then EACInCache MAdd v
+                               else EACFail
     | _ -> EACFail
-  )
+    )
   
-  | EACInCache m k v -> (
+  | EACInCache m v -> (
     match e with 
-    | Get k' v' -> if k' = k && (DVal v') = v then s
-                   else EACFail
-    | Put k' v' -> if k' = k then EACInCache m k (DVal v')
-                   else EACFail 
-    | EvictM k' _ -> if k' = k then EACEvicted MAdd k v
-                     else EACFail
-    | EvictBM k' _ _ -> if k' = k && m = MAdd then EACEvicted BAdd k v
-                        else EACFail
-    | EvictB k' _ -> if k' = k && m = BAdd then EACEvicted BAdd k v
-                     else EACFail
+    | NEvict (Get _ v') -> if (DVal v') = v then s
+                           else EACFail
+    | NEvict (Put _ v') -> EACInCache m (DVal v')                   
+    | Evict (EvictM _ _) v' -> if DVal? v && v' <> v then EACFail
+                               else EACEvicted MAdd v
+    | Evict (EvictBM _ _ _) v' -> if DVal? v && v' <> v || m <> MAdd then EACFail
+                                  else EACEvicted BAdd v
+    | Evict (EvictB _ _) v' ->  if DVal? v && v' <> v || m <> BAdd then EACFail
+                                else EACEvicted BAdd v
     | _ -> EACFail
-  )
+    )
   
-  | EACEvicted m k v -> (
+  | EACEvicted m v -> (
     match e with
-    | AddM (k',v') _ -> if k' = k && v' = v && m = MAdd then EACInCache MAdd k v
-                        else EACFail
-    | AddB (k',v') _ _ -> if k' = k && v' = v && m = BAdd then EACInCache BAdd k v
-                          else EACFail
+    | NEvict (AddM (_,v') _) -> if v' = v && m = MAdd then EACInCache MAdd v
+                                else EACFail
+    | NEvict (AddB (_,v') _ _) -> if v' = v && m = BAdd then EACInCache BAdd v
+                                else EACFail
     | _ -> EACFail
   )
-                                
-let eac_verify (l: vlog) = reduce EACInit eac_add l
 
-let eac_valid (l: vlog) = not (EACFail? (eac_verify l))
+let eac_smk = SeqMachine EACInit EACFail eac_add
 
-let vlog_entry_key (e: vlog_entry) = 
-  match e with
+let to_vlog_entry (ee:vlog_entry_ext) = 
+  match ee with
+  | Evict e _ -> e
+  | NEvict e -> e
+
+let vlog_entry_key (e: vlog_entry_ext) = 
+  match (to_vlog_entry e) with
   | Get k _ -> k
   | Put k _ -> k
   | AddM (k,_) _ -> k
@@ -68,71 +88,13 @@ let vlog_entry_key (e: vlog_entry) =
   | EvictB k _ -> k
   | EvictBM k _ _ -> k
 
-let lemma_eac_fail_sticky ():
-  Lemma (forall (e:vlog_entry). eac_add e EACFail = EACFail) = ()
-
-let rec lemma_eac_valid_implies_prefix (l: vlog{eac_valid l}) (i: nat{i <= length l}):
-  Lemma (requires True)
-        (ensures (eac_valid (prefix l i)))
-        (decreases (length l)) 
-        [SMTPat (prefix l i)]
-        = 
-  let n = length l in
-  if n = 0 then ()
-  else if i = n then ()
-  else 
-    let l' = prefix l (n - 1) in
-    if eac_valid l' then (
-      lemma_eac_valid_implies_prefix l' i;
-      ()
-    )
-    else (
-      lemma_reduce_prefix EACInit eac_add l (n - 1);
-      lemma_reduce_identity EACFail eac_add (suffix l 1)
-    )
-
-let invalid_or_attached_to (k: key) (s: eac_state) =
-  match s with 
-  | EACInit -> false
-  | EACFail -> true
-  | EACInCache _ k' _ -> k' = k
-  | EACEvicted _ k' _ -> k' = k
-
-let lemma_eac_invariant (k: key): 
-  Lemma (forall s. forall e. invalid_or_attached_to k s ==> invalid_or_attached_to k (eac_add e s)) = ()
-
-let lemma_eac_valid_implies_same_key (l: vlog) (i: seq_index l):
-  Lemma (requires eac_valid l /\ length l > 0)
-        (ensures (vlog_entry_key (index l i) = vlog_entry_key (index l 0)))
-        (decreases (length l)) = 
-  let e0 = index l 0 in
-  let k = vlog_entry_key e0 in
-  let li = prefix l (i + 1) in
-  let s0 = eac_verify (prefix l 1) in
-  lemma_eac_valid_implies_prefix l 1;
-  lemma_reduce_singleton EACInit eac_add (prefix l 1);
-  if i = 0 then ()
-  else if i = 1 then (
-    lemma_reduce_prefix EACInit eac_add li 1;
-    lemma_reduce_singleton s0 eac_add (suffix li 1)
-  )
-  else ( 
-    let li' = prefix l i in
-    lemma_reduce_prefix EACInit eac_add li' 1;
-    lemma_reduce_property_closure (invalid_or_attached_to k) s0 eac_add (suffix li' (i - 1));
-    let si' = eac_verify li' in
-    lemma_reduce_prefix EACInit eac_add li i;    
-    lemma_reduce_singleton si' eac_add (suffix li 1)
-  )
-
-(* filter out entries of vlog affecting key k *)
-let key_vlog (k: key) (l: vlog) = filter (fun e -> k = vlog_entry_key e) l
+let eac_sm = PSM eac_smk vlog_entry_key
 
 (* evict add consistency *)
-let eac (l:vlog) = forall (k: key). ~(EACFail? (eac_verify (key_vlog k l)))
+let eac (l:vlog_ext) = valid_all eac_sm l
 
 (* refinement of evict add consistent logs *)
-type eac_log = l:vlog{eac l}
+type eac_log = l:vlog_ext{eac l}
 
 (* the state operations of a vlog *)
 let is_state_op (e: vlog_entry) = 
@@ -151,6 +113,64 @@ let to_state_op (e:vlog_entry {is_state_op e}) =
 let to_state_op_vlog (l: vlog) = 
   map to_state_op (filter_refine is_state_op l)
 
+(* valid eac states *)
+let valid_eac_state (st:eac_state) = not (EACFail? st)
+
+(* value of a valid state *)
+let value_of (st:eac_state {valid_eac_state st}) =
+  match st with
+  | EACInit -> DVal Null
+  | EACInCache _ v -> v
+  | EACEvicted _ v -> v
+
+let to_vlog (l:vlog_ext) = 
+  map to_vlog_entry l
+
+let rec lemma_comm (le:vlog_ext) (k:data_key):
+  Lemma (to_state_op_vlog (to_vlog (partn eac_sm k le)) = 
+         partn ssm k (to_state_op_vlog (to_vlog le))) = 
+  let lek = partn eac_sm k le in
+  let lk = to_vlog lek in
+  let lks = to_state_op_vlog lk in
+  let l = to_vlog le in
+  let ls = to_state_op_vlog l in
+  let lsk = partn ssm k ls in
+  admit()
+
+  
+let lemma_eac_k_implies_ssm_k_valid (le:eac_log) (k:data_key):
+  Lemma (valid ssm_k (to_state_op_vlog (to_vlog (partn eac_sm k le)))) = 
+  let lek = partn eac_sm k le in
+  let lk = to_vlog lek in
+  let lks = to_state_op_vlog lk in
+  if valid ssm_k lks then ()
+  else (
+    let i = max_valid_prefix ssm_k lks in  
+    let op = index lks i in
+    let ssti = seq_machine_run ssm_k (prefix lks (i + 1)) in
+    assert(ssti = StateFail);
+    
+    let ssti' = seq_machine_run ssm_k (prefix lks i) in
+    if i = 0 then (
+      lemma_reduce_singleton StateInit apply_state_op (prefix lks (i + 1));
+      assert(StateFail = apply_state_op op StateInit);
+      assert(Veritas.State.Get? op && Veritas.State.Get?.v op <> Null);
+      admit()
+    )
+    else admit()
+  )
+
 (* evict add consistency implies rw-consistency *)
-let lemma_eac_implies_rw_consistent (l:eac_log):
-  Lemma (rw_consistent (to_state_op_vlog l)) = admit()
+let lemma_eac_implies_rw_consistent (le:eac_log):
+  Lemma (rw_consistent (to_state_op_vlog (to_vlog le))) = 
+  let l = to_vlog le in
+  let s = to_state_op_vlog l in
+  let rwc = valid_all_comp ssm s in
+  lemma_state_sm_equiv_rw_consistent s;
+  if rwc then () // nothing to prove if rw_consistent
+  else (
+    (* invalidating key *)
+    let k: data_key = invalidating_key ssm s in
+    lemma_eac_k_implies_ssm_k_valid le k;    
+    lemma_comm le k
+  )
